@prefix rdfs:    <http://www.w3.org/2000/01/rdf-schema#> .
@prefix owl:     <http://www.w3.org/2002/07/owl#> .
@prefix xsd:     <http://www.w3.org/2001/XMLSchema#> .
@prefix rdf:     <http://www.w3.org/1999/02/22-rdf-syntax-ns#> .

<http://purl.org/olia/stanford.owl#DependencyLabel>
      a       owl:Class ;
      rdfs:subClassOf <http://purl.org/olia/system.owl#Feature> .

owl:Thing
      a       owl:Class .

<http://purl.org/olia/stanford.owl#Object>
      a       owl:Class ;
      rdfs:label "object" ;
      rdfs:subClassOf <http://purl.org/olia/stanford.owl#Complement> .

<http://purl.org/olia/stanford.owl#Dependent>
      a       owl:Class ;
      rdfs:comment "dependencies are established between tokens, i.e., exactly those entities that are subject to part of speech annotation" ;
      rdfs:label "dependent" ;
      rdfs:subClassOf <http://purl.org/olia/stanford.owl#DependencyLabel> .

<http://purl.org/olia/stanford.owl#pobj>
      a       owl:Thing .

<http://purl.org/olia/stanford.owl#ObjectOfPreposition>
      a       owl:Class ;
      rdfs:label "object of preposition" ;
      rdfs:subClassOf <http://purl.org/olia/stanford.owl#Object> .

<http://purl.org/olia/system.owl#LinguisticAnnotation>
      a       owl:Class ;
      rdfs:comment "Linguistic annotations pertain to either structural entities (words, tokens, constituents, sentences => UnitOfAnnotation), relations between these (dependency, dominance, coreference, etc. => Relation), or grammatical features attached to these (case, gender, number, agreement, tense, mood, aspect, ... => Feature)." ;
      rdfs:subClassOf owl:Thing .

<http://purl.org/olia/system.owl#Feature>
      a       owl:Class ;
      rdfs:comment "UnitsOfAnnotation and Relations can be described in a more detailed way by the features that are attached to them, e.g., case, number, or aspect. Features are, however, not subject to further annotations (by means of hasFeature), they are thus disjoint from Relations and UnitsOfAnnotation." ;
      rdfs:subClassOf <http://purl.org/olia/system.owl#LinguisticAnnotation> .

<http://purl.org/olia/stanford.owl#Argument>
      a       owl:Class ;
      rdfs:label "argument" ;
      rdfs:subClassOf <http://purl.org/olia/stanford.owl#Dependent> .

<http://purl.org/olia/stanford.owl#Complement>
      a       owl:Class ;
      rdfs:label "complement" ;
      rdfs:subClassOf <http://purl.org/olia/stanford.owl#Argument> .
