<rdf:RDF
    xmlns:rdf="http://www.w3.org/1999/02/22-rdf-syntax-ns#"
    xmlns:owl="http://www.w3.org/2002/07/owl#"
    xmlns:xsd="http://www.w3.org/2001/XMLSchema#"
    xmlns:rdfs="http://www.w3.org/2000/01/rdf-schema#" > 
  <rdf:Description rdf:about="http://purl.org/olia/olia-top.owl#SemanticFeature">
    <rdf:type rdf:resource="http://www.w3.org/2002/07/owl#Class"/>
    <rdfs:subClassOf rdf:resource="http://purl.org/olia/system.owl#Feature"/>
    <rdfs:subClassOf rdf:resource="http://purl.org/olia/olia-top.owl#LinguisticConcept"/>
    <rdfs:comment></rdfs:comment>
  </rdf:Description>
  <rdf:Description rdf:about="http://purl.org/olia/brown.owl#Negator">
    <rdf:type rdf:resource="http://www.w3.org/2002/07/owl#Class"/>
    <rdfs:comment>The word "not" is tagged *, which is joined to the verb tag in the case of contracted forms.</rdfs:comment>
    <rdfs:subClassOf rdf:resource="http://purl.org/olia/olia.owl#Negation"/>
    <rdfs:subClassOf rdf:resource="http://purl.org/olia/brown.owl#Tag"/>
  </rdf:Description>
  <rdf:Description rdf:about="http://www.w3.org/2002/07/owl#Thing">
    <rdf:type rdf:resource="http://www.w3.org/2002/07/owl#Class"/>
  </rdf:Description>
  <rdf:Description rdf:about="http://purl.org/olia/olia-top.owl#LinguisticConcept">
    <rdfs:comment>The OLiA ontology specifies linguistic concepts on a theoretical basis, as for concepts used in annotations, see system.owl.
There is a great extent of overlap between LinguisticCategories/LinguisticFeatures and Categories/Features as defined in system.owl.</rdfs:comment>
    <rdfs:subClassOf rdf:resource="http://www.w3.org/2002/07/owl#Thing"/>
    <rdf:type rdf:resource="http://www.w3.org/2002/07/owl#Class"/>
  </rdf:Description>
  <rdf:Description rdf:about="http://purl.org/olia/olia-top.owl#PolarityFeature">
    <rdfs:subClassOf rdf:resource="http://purl.org/olia/olia-top.owl#SemanticFeature"/>
    <rdf:type rdf:resource="http://www.w3.org/2002/07/owl#Class"/>
  </rdf:Description>
  <rdf:Description rdf:about="http://purl.org/olia/system.owl#UnitOfAnnotation">
    <rdfs:comment>A UnitOfAnnotation is a structural entity that can be annotated, e.g., a word, token, constituent, or another types of markable.
Word classes, etc., are then modelled as indirect children of UnitOfAnnotation. The division between Features and classes of UnitsOfAnnotation follows conventional standards.
    </rdfs:comment>
    <rdfs:subClassOf rdf:resource="http://purl.org/olia/system.owl#LinguisticAnnotation"/>
    <rdf:type rdf:resource="http://www.w3.org/2002/07/owl#Class"/>
  </rdf:Description>
  <rdf:Description rdf:about="http://purl.org/olia/system.owl#LinguisticAnnotation">
    <rdf:type rdf:resource="http://www.w3.org/2002/07/owl#Class"/>
    <rdfs:subClassOf rdf:resource="http://www.w3.org/2002/07/owl#Thing"/>
    <rdfs:comment>Linguistic annotations pertain to either structural entities (words, tokens, constituents, sentences =&gt; UnitOfAnnotation), relations between these (dependency, dominance, coreference, etc. =&gt; Relation), or grammatical features attached to these (case, gender, number, agreement, tense, mood, aspect, ... =&gt; Feature).</rdfs:comment>
  </rdf:Description>
  <rdf:Description rdf:about="http://purl.org/olia/olia.owl#Negation">
    <rdf:type rdf:resource="http://www.w3.org/2002/07/owl#Class"/>
    <rdfs:subClassOf rdf:resource="http://purl.org/olia/olia-top.owl#PolarityFeature"/>
    <rdfs:comment>http://purl.org/olia/mte/multext-east.owl#Negated: Negative="yes" encodes negative verbal word-forms in Slavic languages and Estonian. (MTE v4) 
    	In Slovak, for example, verbs form negative by prefix 'ne-', with the exception of the verb "byť" (E. "to be") which forms the negative in indicative by using separate particle "nie", e.g. "nie je" (is not). Here, Slovak "je" would be marked as negative, despite having positive form. In Resian, negative is always marked as 'n' except for two verbs: 'nïman' / not to have, 'nïsi' / not to be. (MTE v4)</rdfs:comment>
  </rdf:Description>
  <rdf:Description rdf:about="http://purl.org/olia/brown.owl#Tag">
    <rdf:type rdf:resource="http://www.w3.org/2002/07/owl#Class"/>
    <rdfs:subClassOf rdf:resource="http://purl.org/olia/system.owl#UnitOfAnnotation"/>
  </rdf:Description>
  <rdf:Description rdf:about="http://purl.org/olia/brown.owl#negator">
    <rdf:type rdf:resource="http://www.w3.org/2002/07/owl#Thing"/>
  </rdf:Description>
  <rdf:Description rdf:about="http://purl.org/olia/system.owl#Feature">
    <rdfs:comment>UnitsOfAnnotation and Relations can be described in a more detailed way by the features that are attached to them, e.g., case, number, or aspect. Features are, however, not subject to further annotations (by means of hasFeature), they are thus disjoint from Relations and UnitsOfAnnotation.</rdfs:comment>
    <rdfs:subClassOf rdf:resource="http://purl.org/olia/system.owl#LinguisticAnnotation"/>
    <rdf:type rdf:resource="http://www.w3.org/2002/07/owl#Class"/>
  </rdf:Description>
</rdf:RDF>
