@prefix rdfs:    <http://www.w3.org/2000/01/rdf-schema#> .
@prefix owl:     <http://www.w3.org/2002/07/owl#> .
@prefix xsd:     <http://www.w3.org/2001/XMLSchema#> .
@prefix rdf:     <http://www.w3.org/1999/02/22-rdf-syntax-ns#> .

owl:Thing
      a       owl:Class .

<http://purl.org/olia/brown.owl#TL>
      a       owl:Thing .

<http://purl.org/olia/system.owl#UnitOfAnnotation>
      a       owl:Class ;
      rdfs:comment """A UnitOfAnnotation is a structural entity that can be annotated, e.g., a word, token, constituent, or another types of markable.
Word classes, etc., are then modelled as indirect children of UnitOfAnnotation. The division between Features and classes of UnitsOfAnnotation follows conventional standards.
    """ ;
      rdfs:subClassOf <http://purl.org/olia/system.owl#LinguisticAnnotation> .

<http://purl.org/olia/system.owl#LinguisticAnnotation>
      a       owl:Class ;
      rdfs:comment "Linguistic annotations pertain to either structural entities (words, tokens, constituents, sentences => UnitOfAnnotation), relations between these (dependency, dominance, coreference, etc. => Relation), or grammatical features attached to these (case, gender, number, agreement, tense, mood, aspect, ... => Feature)." ;
      rdfs:subClassOf owl:Thing .

<http://purl.org/olia/brown.owl#TitleWord>
      a       owl:Class ;
      rdfs:comment """These are words occurring as constituents of titles, e.g. of books, plays, corporations, government agencies, etc., are given their normal tag with the addition of the hyphenated tag -TL.
In most cases these words are capitalized, except for function-words such as prepositions, conjunctions, and sometimes pronouns. 
Some examples: 
 the United 	States 	of 	America
 VBN-TL 	NNS-TL 	IN-TL 	NP-TL

Gulliver's 	Travels
NP$-TL 	NNS-TL

But the titles Mr , Mrs., and Miss and Sir have been tagged as proper noun.""" ;
      rdfs:subClassOf <http://purl.org/olia/brown.owl#Tag> .

<http://purl.org/olia/brown.owl#Tag>
      a       owl:Class ;
      rdfs:subClassOf <http://purl.org/olia/system.owl#UnitOfAnnotation> .
